Verify saturn/mpsc_latch1.

theories/saturn/mpsc_latch1.v
@@ -1,13 +1,20 @@
 From zebre Require Import
   prelude.
+From zebre.iris.base_logic Require Import
+  lib.oneshot
+  lib.excl.
 From zebre.language Require Import
-  notations.
+  notations
+  diaframe.
 From zebre.std Require Import
   condition.
 From zebre.saturn Require Export
   base.
 From zebre Require Import
   options.
+
+Implicit Types b : bool.
+Implicit Types l : location.
 
 #[local] Notation "'flag'" := (
   in_type "t" 0
@@ -24,10 +31,10 @@ From zebre Require Import
 
 Definition mpsc_latch1_create : val :=
   λ: <>,
-    let: "t" := { #false; (); () } in
-    "t" <-{mutex} mutex_create () ;;
-    "t" <-{condition} condition_create () ;;
-    "t".
+    { #false;
+      mutex_create ();
+      condition_create ()
+    }.
 
 Definition mpsc_latch1_signal : val :=
   λ: "t",
@@ -48,14 +55,324 @@ Definition mpsc_latch1_signal : val :=
       "res"
     ).
 
+Definition mpsc_latch1_try_wait : val :=
+  λ: "t",
+    "t".{flag}.
+
 Definition mpsc_latch1_wait : val :=
   λ: "t",
-    let: "mtx" := "t".{mutex} in
-    let: "cond" := "t".{condition} in
-    mutex_protect "mtx" (λ: <>,
-      condition_wait_until "cond" "mtx" (λ: <>, "t".{flag})
+    ifnot: mpsc_latch1_try_wait "t" then (
+      let: "mtx" := "t".{mutex} in
+      let: "cond" := "t".{condition} in
+      mutex_protect "mtx" (λ: <>,
+        condition_wait_until "cond" "mtx" (λ: <>, "t".{flag})
+      )
     ).
 
+Class MpscLatch1G Σ `{zebre_G : !ZebreG Σ} := {
+  #[local] mpsc_latch1_G_mutex_G :: MutexG Σ ;
+  #[local] mpsc_latch1_G_lstate_G :: OneshotG Σ unit unit ;
+  #[local] mpsc_latch1_G_consumer_G :: ExclG Σ unitO ;
+}.
+
+Definition mpsc_latch1_Σ := #[
+  mutex_Σ ;
+  oneshot_Σ unit unit ;
+  excl_Σ unitO
+].
+#[global] Instance subG_mpsc_latch1_Σ Σ `{zebre_G : !ZebreG Σ} :
+  subG mpsc_latch1_Σ Σ →
+  MpscLatch1G Σ .
+Proof.
+  solve_inG.
+Qed.
+
+Section mpsc_latch1_G.
+  Context `{mpsc_latch1_G : MpscLatch1G Σ}.
+
+  Record mpsc_latch1_meta := {
+    mpsc_latch1_meta_lstate : gname ;
+    mpsc_latch1_meta_consumer : gname ;
+  }.
+  Implicit Types γ : mpsc_latch1_meta.
+
+  #[local] Instance mpsc_latch1_meta_eq_dec : EqDecision mpsc_latch1_meta :=
+    ltac:(solve_decision).
+  #[local] Instance mpsc_latch1_meta_countable :
+    Countable mpsc_latch1_meta.
+  Proof.
+    pose encode γ := (
+      γ.(mpsc_latch1_meta_lstate),
+      γ.(mpsc_latch1_meta_consumer)
+    ).
+    pose decode := λ '(γ_lstate, γ_consumer), {|
+      mpsc_latch1_meta_lstate := γ_lstate ;
+      mpsc_latch1_meta_consumer := γ_consumer ;
+    |}.
+    refine (inj_countable' encode decode _). intros []. done.
+  Qed.
+
+  #[local] Definition mpsc_latch1_inv_inner l γ P : iProp Σ :=
+    ∃ b,
+    l.[flag] ↦ #b ∗
+    if b then
+      oneshot_shot γ.(mpsc_latch1_meta_lstate) () ∗
+      (P ∨ excl γ.(mpsc_latch1_meta_consumer) ())
+    else
+      oneshot_pending γ.(mpsc_latch1_meta_lstate) (DfracOwn 1) ().
+  #[local] Definition mpsc_latch1_inv t P : iProp Σ :=
+    ∃ l γ mtx cond,
+    ⌜t = #l⌝ ∗
+    meta l nroot γ ∗
+    l.[mutex] ↦□ mtx ∗
+    mutex_inv mtx True ∗
+    l.[condition] ↦□ cond ∗
+    condition_inv cond ∗
+    inv nroot (mpsc_latch1_inv_inner l γ P).
+
+  Definition mpsc_latch1_consumer t : iProp Σ :=
+    ∃ l γ,
+    ⌜t = #l⌝ ∗
+    meta l nroot γ ∗
+    excl γ.(mpsc_latch1_meta_consumer) ().
+
+  Definition mpsc_latch1_signaled t : iProp Σ :=
+    ∃ l γ,
+    ⌜t = #l⌝ ∗
+    meta l nroot γ ∗
+    oneshot_shot γ.(mpsc_latch1_meta_lstate) ().
+
+  #[global] Instance mpsc_latch1_inv_contractive t :
+    Contractive (mpsc_latch1_inv t).
+  Proof.
+    rewrite /mpsc_latch1_inv /mpsc_latch1_inv_inner. solve_contractive.
+  Qed.
+  #[global] Instance mpsc_latch1_inv_ne t :
+    NonExpansive (mpsc_latch1_inv t).
+  Proof.
+    apply _.
+  Qed.
+  #[global] Instance mpsc_latch1_inv_proper t :
+    Proper ((≡) ==> (≡)) (mpsc_latch1_inv t).
+  Proof.
+    apply _.
+  Qed.
+
+  #[global] Instance mpsc_latch1_inv_persistent t P :
+    Persistent (mpsc_latch1_inv t P).
+  Proof.
+    apply _.
+  Qed.
+  #[global] Instance mpsc_latch1_signaled_persistent t :
+    Persistent (mpsc_latch1_signaled t).
+  Proof.
+    apply _.
+  Qed.
+  #[global] Instance mpsc_latch1_consumer_timeless t :
+    Timeless (mpsc_latch1_consumer t).
+  Proof.
+    apply _.
+  Qed.
+
+  Lemma mpsc_latch1_consumer_exclusive t :
+    mpsc_latch1_consumer t -∗
+    mpsc_latch1_consumer t -∗
+    False.
+  Proof.
+    iIntros "(%l & %γ & -> & #Hmeta & Hconsumer1) (%_l & %_γ & %Heq & _Hmeta & Hconsumer2)". injection Heq as <-.
+    iDestruct (meta_agree with "Hmeta _Hmeta") as %<-. iClear "_Hmeta".
+    iApply (excl_exclusive with "Hconsumer1 Hconsumer2").
+  Qed.
+
+  Lemma mpsc_latch1_create_spec P :
+    {{{ True }}}
+      mpsc_latch1_create ()
+    {{{ t,
+      RET t;
+      mpsc_latch1_inv t P ∗
+      mpsc_latch1_consumer t
+    }}}.
+  Proof.
+    iIntros "%Φ _ HΦ".
+
+    wp_rec.
+    wp_smart_apply (mutex_create_spec True with "[//]") as "%mtx #Hmtx_inv".
+    wp_smart_apply (condition_create_spec _ with "[//]") as "%cond #Hcond_inv".
+    wp_record l as "Hmeta" "(Hflag & Hmtx & Hcond & _)".
+    iMod (pointsto_persist with "Hmtx") as "Hmtx".
+    iMod (pointsto_persist with "Hcond") as "Hcond".
+
+    iMod (oneshot_alloc ()) as "(%γ_lstate & Hpending)".
+
+    iMod (excl_alloc (excl_G := mpsc_latch1_G_consumer_G) ()) as "(%γ_consumer & Hconsumer)".
+
+    pose γ := {|
+      mpsc_latch1_meta_lstate := γ_lstate ;
+      mpsc_latch1_meta_consumer := γ_consumer ;
+    |}.
+    iMod (meta_set _ _ γ with "Hmeta") as "#Hmeta"; first done.
+
+    iSteps.
+  Qed.
+
+  Lemma mpsc_latch1_signal_spec t P :
+    {{{
+      mpsc_latch1_inv t P ∗
+      P
+    }}}
+      mpsc_latch1_signal t
+    {{{ b,
+      RET #b;
+      mpsc_latch1_signaled t
+    }}}.
+  Proof.
+    iIntros "%Φ ((%l & %γ & %mtx & %cond & -> & #Hmeta & #Hmtx & #Hmtx_inv & #Hcond & #Hcond_inv & #Hinv) & HP) HΦ".
+
+    wp_rec.
+    wp_pures.
+
+    wp_bind (!_)%E.
+    iInv "Hinv" as "(%b & Hflag & Hb)".
+    wp_load.
+    destruct b; first iSteps.
+    iSplitR "HP HΦ"; first iSteps.
+    iModIntro.
+
+    wp_load.
+    pose (Ψ_mtx res := (
+      ∃ b,
+      ⌜res = #b⌝ ∗
+      oneshot_shot γ.(mpsc_latch1_meta_lstate)  ()
+    )%I).
+    wp_smart_apply (mutex_protect_spec Ψ_mtx with "[$Hmtx_inv HP]"); last first.
+    { iSteps. iModIntro.
+      wp_apply (condition_broadcast_spec with "Hcond_inv").
+      iSteps.
+    }
+    iIntros "Hmtx_locked _".
+    wp_pures.
+
+    wp_bind (!_)%E.
+    iInv "Hinv" as "(%b & Hflag & Hb)".
+    wp_load.
+    destruct b; first iSteps.
+    iSplitR "HP Hmtx_locked"; first iSteps.
+    iModIntro.
+
+    wp_pures.
+
+    wp_bind (_ <- _)%E.
+    iInv "Hinv" as "(%b & Hflag & Hb)".
+    wp_store.
+    destruct b; first iSteps.
+    iMod (oneshot_update_shot with "Hb") as "#Hshot".
+    iSteps.
+  Qed.
+
+  Lemma mpsc_latch1_try_wait_spec_signaled t P :
+    {{{
+      mpsc_latch1_inv t P ∗
+      mpsc_latch1_consumer t ∗
+      mpsc_latch1_signaled t
+    }}}
+      mpsc_latch1_try_wait t
+    {{{
+      RET #true;
+      P
+    }}}.
+  Proof.
+    iIntros "%Φ ((%l & %γ & %mtx & %cond & -> & #Hmeta & #Hmtx & #Hmtx_inv & #Hcond & #Hcond_inv & #Hinv) & (%_l1 & %_γ1 & %Heq1 & _Hmeta1 & Hconsumer) & (%_l2 & %_γ2 & %Heq2 & _Hmeta2 & #Hshot)) HΦ". injection Heq1 as <-. injection Heq2 as <-.
+    iDestruct (meta_agree with "Hmeta _Hmeta1") as %<-. iClear "_Hmeta1".
+    iDestruct (meta_agree with "Hmeta _Hmeta2") as %<-. iClear "_Hmeta2".
+
+    wp_rec.
+    wp_pures.
+
+    iInv "Hinv" as "(%b & Hflag & Hb)".
+    wp_load.
+    destruct b.
+
+    - iDestruct "Hb" as "(_ & [Hmodel | Hconsumer'])"; first iSmash.
+      iDestruct (excl_exclusive with "Hconsumer Hconsumer'") as %[].
+
+    - iDestruct (oneshot_pending_shot with "Hb Hshot") as %[].
+  Qed.
+  Lemma mpsc_latch1_try_wait_spec t P :
+    {{{
+      mpsc_latch1_inv t P ∗
+      mpsc_latch1_consumer t
+    }}}
+      mpsc_latch1_try_wait t
+    {{{ b,
+      RET #b;
+      if b then
+        P
+      else
+        mpsc_latch1_consumer t
+    }}}.
+  Proof.
+    iIntros "%Φ ((%l & %γ & %mtx & %cond & -> & #Hmeta & #Hmtx & #Hmtx_inv & #Hcond & #Hcond_inv & #Hinv) & (%_l & %_γ & %Heq & _Hmeta & Hconsumer)) HΦ". injection Heq as <-.
+    iDestruct (meta_agree with "Hmeta _Hmeta") as %<-. iClear "_Hmeta".
+
+    wp_rec.
+    wp_pures.
+
+    iInv "Hinv" as "(%b & Hflag & Hb)".
+    wp_load.
+    destruct b; last iSteps.
+    iDestruct "Hb" as "(Hshot & [Hmodel | Hconsumer'])"; first iSmash.
+    iDestruct (excl_exclusive with "Hconsumer Hconsumer'") as %[].
+  Qed.
+
+  Lemma mpsc_latch1_wait_spec t P :
+    {{{
+      mpsc_latch1_inv t P ∗
+      mpsc_latch1_consumer t
+    }}}
+      mpsc_latch1_wait t
+    {{{
+      RET ();
+      P
+    }}}.
+  Proof.
+    iIntros "%Φ (#Hinv & Hconsumer) HΦ".
+
+    wp_rec.
+    wp_apply (mpsc_latch1_try_wait_spec with "[$Hinv $Hconsumer]") as ([]) "Hconsumer"; first iSteps.
+
+    iDestruct "Hinv" as "(%l & %γ & %mtx & %cond & -> & #Hmeta & #Hmtx & #Hmtx_inv & #Hcond & #Hcond_inv & #Hinv)".
+    iDestruct "Hconsumer" as "(%_l & %_γ & %Heq & _Hmeta & Hconsumer)". injection Heq as <-.
+    iDestruct (meta_agree with "Hmeta _Hmeta") as %<-. iClear "_Hmeta".
+
+    do 2 wp_load.
+    pose Ψ_mtx res := (
+      ⌜res = ()%V⌝ ∗
+      P
+    )%I.
+    wp_smart_apply (mutex_protect_spec Ψ_mtx with "[$Hmtx_inv Hconsumer]"); last iSteps.
+    iIntros "Hmtx_locked _".
+    pose (Ψ_cond b := (
+      if b then
+        P
+      else
+        excl γ.(mpsc_latch1_meta_consumer) ()
+    )%I).
+    wp_smart_apply (condition_wait_until_spec Ψ_cond with "[$Hcond_inv $Hmtx_inv $Hmtx_locked $Hconsumer]"); last iSteps.
+    clear. iIntros "!> %Φ (Hmtx_locked & _ & Hconsumer) HΦ".
+    wp_pures.
+    iInv "Hinv" as "(%b & Hflag & Hb)".
+    wp_load.
+    destruct b; last iSteps.
+    iDestruct "Hb" as "(Hshot & [Hmodel | Hconsumer'])"; first iSmash.
+    iDestruct (excl_exclusive with "Hconsumer Hconsumer'") as %[].
+  Qed.
+End mpsc_latch1_G.
+
 #[global] Opaque mpsc_latch1_create.
-#[global] Opaque mpsc_latch1_wait.
 #[global] Opaque mpsc_latch1_signal.
+#[global] Opaque mpsc_latch1_try_wait.
+#[global] Opaque mpsc_latch1_wait.
+
+#[global] Opaque mpsc_latch1_inv.
+#[global] Opaque mpsc_latch1_consumer.
+#[global] Opaque mpsc_latch1_signaled.
